formalization/eitt.v
@@ -1,0 +1,22 @@
+(* The target type theory, economic itensional type theory *)
+
+Require config.
+Require Import tt.
+
+Section Eitt.
+
+Local Instance hasPrecond : config.Precond
+  := {| config.precondFlag := config.No |}.
+Local Instance hasReflection : config.Reflection
+  := {| config.reflectionFlag := config.No |}.
+
+Definition isctx := isctx.
+Definition issubst := issubst.
+Definition istype := istype.
+Definition isterm := isterm.
+Definition eqctx := eqctx.
+Definition eqsubst := eqsubst.
+Definition eqtype := eqtype.
+Definition eqterm := eqterm.
+
+End Eitt.
